src/Pipit.Exp.Causality.fst
@@ -49,7 +49,7 @@ let rec direct_dependency (#t: table) (#c: context t) (#a: t.ty) (e: exp t c a) 
   (* Should we care if a contract's relies or guarantees mention `i`?
      I don't think it's strictly necessary - causality is required for total evaluation, which
      uses the implementation rather than the abstraction. *)
-  | XContract rely guar impl ->
+  | XContract _ rely guar impl ->
     direct_dependency rely i ||
     direct_dependency impl i ||
     direct_dependency impl i
@@ -78,7 +78,7 @@ let rec causal (#t: table) (#c: context t) (#a: t.ty) (e: exp t c a): Tot bool (
   | XMu e1 -> causal e1 && not (direct_dependency e1 0)
   | XLet b e1 e2 -> causal e1 && causal e2
   | XCheck _ e1 -> causal e1
-  | XContract rely guar impl ->
+  | XContract _ rely guar impl ->
     causal rely && causal guar && causal impl
 
 and causal_apps (#t: table) (#c: context t) (#a: funty t.ty) (e: exp_apps t c a): Tot bool (decreases e) =
