src/Pipit.Exp.Checked.Base.fst
@@ -1,0 +1,172 @@
+(* Checked expressions: expressions that are known to satisfy properties
+*)
+module Pipit.Exp.Checked.Base
+
+open Pipit.Prim.Table
+
+open Pipit.Exp.Base
+open Pipit.Exp.Bigstep
+open Pipit.Exp.Binding
+open Pipit.Exp.Causality
+
+module C  = Pipit.Context.Base
+module CR = Pipit.Context.Row
+module CP = Pipit.Context.Properties
+
+module PM = Pipit.Prop.Metadata
+
+// Which is better: inductive relation or recursive definition?
+// noeq
+// type check (mode: check_mode) (#t: table) (#c: context t): (#a: t.ty) -> list (row c) -> exp t c a -> Type =
+//  | CkBase:
+//           #valty: t.ty ->
+//           streams: list (row c)    ->
+//           e: exp_base t c valty    ->
+//           check mode streams (XBase e)
+//  | CkApps:
+//           #valty: t.ty ->
+//           streams: list (row c)    ->
+//           e: exp_apps t c (FTVal valty)    ->
+//           check_apps mode streams e ->
+//           check mode streams (XApps e)
+//  | CkFby1: #a: t.ty                ->
+//            start: list (row c) { List.Tot.length start <= 1 }
+//                                    ->
+//            v0: t.ty_sem a          ->
+//            e: exp t c a            ->
+//            check mode start (XFby v0 e)
+//  | CkFbyS: #a: t.ty                 ->
+//            latest: row c            ->
+//            prefix: list (row c) { List.Tot.length prefix >= 1 }
+//                                     ->
+//            v0: t.ty_sem a           ->
+//            e: exp t c a             ->
+//            check mode            prefix           e ->
+//            check mode (latest :: prefix) (XFby v0 e)
+
+//  | CkMu: #valty: t.ty                         ->
+//          streams: list (row c)                ->
+//          e: exp t (C.close1 c valty) valty    ->
+//          check mode streams (subst1 e (XMu e))     ->
+//          check mode streams (XMu e)
+//  | CkLet:
+//           #a: t.ty -> #b: t.ty                ->
+//           streams: list (row c)               ->
+//           e1: exp t c b                       ->
+//           e2: exp t (C.close1 c b) a          ->
+//           check mode streams (subst1 e2 e1)        ->
+//           check mode streams (XLet b e1 e2)
+
+//  | CkContract:
+//           #valty: t.ty                        ->
+//           streams: list (row c)               ->
+//           status: contract_status             ->
+//           rely: exp t c            t.propty   ->
+//           guar: exp t (valty :: c) t.propty   ->
+//           impl: exp t c            valty      ->
+//           check mode streams rely                  ->
+//           check mode streams (subst1 guar impl)    ->
+//           check mode streams impl                  ->
+//           (Some status.contract_env = mode.check_contract_env ==> bigstep_always streams rely) ->
+//           (Some status.contract_impl = mode.check_contract_impl ==> bigstep_contract_valid streams rely guar impl) ->
+//           check mode streams (XContract status rely guar impl)
+
+//  | CkCheck:
+//           streams: list (row c)                   ->
+//           status:  prop_status                    ->
+//           eprop:   exp t c             t.propty   ->
+//           check mode streams                eprop      ->
+//           (Some status = mode.check_assert ==> bigstep_always streams eprop) ->
+//           check mode streams (XCheck status eprop)
+
+// and check_apps (mode: check_mode) (#t: table) (#c: context t): (#a: funty t.ty) -> list (row c) -> exp_apps t c a -> Type =
+//  (* Primitives `p` are looked up in the primitive table semantics *)
+//  | CkPrim:
+//           streams: list (row c) ->
+//           p: t.prim             ->
+//           check_apps mode streams (XPrim p)
+
+//  (* Element-wise application *)
+//  | CkApp: streams: list (row c)       ->
+//           #a: t.ty -> #b: funty t.ty  ->
+//           f: exp_apps t c (FTFun a b) ->
+//           e: exp t c  a               ->
+//           check_apps mode streams f        ->
+//           check      mode streams e        ->
+//           check_apps mode streams (XApp f e)
+
+
+
+let rec check (#t: table) (#c: context t) (#a: t.ty) (#streams: list (row c)) (#e: exp t c a) (#v: t.ty_sem a)  (mode: PM.check_mode)
+(hBS: bigstep streams e v): Tot prop (decreases hBS) =
+  match hBS with
+  | BSBase _ _ _ _ ->
+    True
+  | BSApps _ _ _ hBSA' ->
+    check_apps mode hBSA'
+  | BSFby1 _ _ _ ->
+    True
+  | BSFbyS _ _ _ _ _ hBS' ->
+    check mode hBS'
+  | BSMu _ _ _ hBS' ->
+    check mode hBS'
+  | BSLet _ _ _ _ hBS' ->
+    check mode hBS'
+  | BSContract _ status rely guar impl _ _ _ hBSr' hBSg' hBSi' ->
+    check mode hBSr' /\
+    check mode hBSg' /\
+    check mode hBSi' /\
+    (PM.prop_status_contains mode status.contract_env ==>
+      bigstep_always streams rely) /\
+    (PM.prop_status_contains mode status.contract_impl ==>
+      bigstep_always streams rely ==>
+      bigstep_always streams (subst1 guar impl))
+  | BSCheck _ status eprop _ hBS' ->
+    check mode hBS' /\
+    (PM.prop_status_contains mode status ==>
+      bigstep_always streams eprop)
+
+and check_apps (#t: table) (#c: context t) (#a: funty t.ty) (#streams: list (row c)) (#e: exp_apps t c a) (#v: funty_sem t.ty_sem a) (mode: PM.check_mode) (hBSA: bigstep_apps streams e v): Tot prop (decreases hBSA) =
+  match hBSA with
+  | BSPrim _ _ -> True
+  | BSApp _ _ _ _ _ hBSA' hBS' -> check_apps mode hBSA' /\ check mode hBS'
+
+let check' (#t: table) (#c: context t) (#a: t.ty) (mode: PM.check_mode) (e: exp t c a) =
+  forall (streams: list (row c)) (v: t.ty_sem a) (hBS: bigstep streams e v).
+    check mode hBS
+
+let check_apps' (#t: table) (#c: context t) (#a: funty t.ty) (mode: PM.check_mode) (e: exp_apps t c a) =
+  forall (streams: list (row c)) (v: funty_sem t.ty_sem a) (hBS: bigstep_apps streams e v).
+    check_apps mode hBS
+
+let bigstep_equivalent (#t: table) (#c: context t) (#a: t.ty) (e e': exp t c a): prop =
+  forall (streams: list (row c)) (v: t.ty_sem a).
+    bigstep streams e v <==> bigstep streams e' v
+
+let check_equivalent (#t: table) (#c: context t) (#a: t.ty) (m m': PM.check_mode) (e e': exp t c a): prop =
+  forall (streams: list (row c)) (v: t.ty_sem a) (hBS: bigstep streams e v).
+    check m hBS <==> check m' hBS
+
+let bless_equivalent (#t: table) (#c: context t) (#a: t.ty) (e e': exp t c a): prop =
+  bigstep_equivalent e e' /\
+  check_equivalent PM.check_mode_all  PM.check_mode_valid   e e' /\
+  check_equivalent PM.check_mode_none PM.check_mode_unknown e e'
+
+let rec bless (#t: table) (#c: context t) (#a: t.ty) (e: exp t c a): Tot (exp t c a) (decreases e) =
+  match e with
+  | XBase _ -> e
+  | XApps e1 -> XApps (bless_apps e1)
+  | XFby v e1 -> XFby v (bless e1)
+  | XMu e1 -> XMu (bless e1)
+  | XLet b e1 e2 -> XLet b (bless e1) (bless e2)
+  | XCheck s e1 -> XCheck PM.PSValid (bless e1)
+  | XContract s r g i ->
+    XContract ({ contract_env = s.contract_env; contract_impl = PM.PSValid })
+      (bless r)
+      (bless g)
+      (bless i)
+
+and bless_apps (#t: table) (#c: context t) (#a: funty t.ty) (e: exp_apps t c a): Tot (exp_apps t c a) (decreases e) =
+  match e with
+  | XPrim p -> XPrim p
+  | XApp f e -> XApp (bless_apps f) (bless e)
