src/Pipit.Prop.Metadata.fst
@@ -1,0 +1,45 @@
+(* Definition of metadata about program properties:
+   so far we only distinguish between properties that have already been checked, and those that should be checked.
+   In the future we may want admitted properties too (which should be trusted but not checked). *)
+module Pipit.Prop.Metadata
+
+(* Status of properties:
+   valid:   property that has been verified to hold
+   unknown: property that is yet to be verified *)
+type prop_status = | PSValid | PSUnknown
+
+(* Status of contracts:
+   contract_impl: if PSValid, then implementation has been verified to satisfy guarantees
+   contract_env: if PSValid, then environment has been verified to satisfiy relies *)
+type contract_status = {
+  contract_impl: prop_status;
+  contract_env:  prop_status;
+}
+
+let contract_status_unknown: contract_status = { contract_impl = PSUnknown; contract_env = PSUnknown }
+
+(* set of prop_status
+   The definition of "checking" a property is parameterised by which kinds of properties one is interested in.
+   It helps to have a first-order representation of a set of property kinds.
+ *)
+type prop_status_set = {
+  prop_status_valid:   bool;
+  prop_status_unknown: bool;
+}
+
+let prop_status_contains (s: prop_status_set) (p: prop_status): bool =
+ match p with
+ | PSValid   -> s.prop_status_valid
+ | PSUnknown -> s.prop_status_unknown
+
+type check_mode = prop_status_set
+// type check_mode = {
+//   check_set:           prop_status_set;
+//   check_contract_impl: prop_status_set;
+//   check_contract_env:  prop_status_set;
+// }
+
+let check_mode_none:    check_mode = { prop_status_valid = false; prop_status_unknown = false; }
+let check_mode_valid:   check_mode = { prop_status_valid = true;  prop_status_unknown = false; }
+let check_mode_unknown: check_mode = { prop_status_valid = false; prop_status_unknown = true; }
+let check_mode_all:     check_mode = { prop_status_valid = true;  prop_status_unknown = true; }
